src/proof/controllers/statefulset/progress.v
@@ -335,7 +335,7 @@ Proof.
   iEval (rewrite -Hmissing_pvcs) in "Hreserved_pvc_frags".
   wp_auto.
   wp_apply (wp_reconcileReplicas_progress γ l set_l good_sl set
-    good_ptrs good_pods pvcs 1 pod_dq Quiescent
+    good_ptrs good_pods pvcs 1 pod_dq terminating_children.No
     with "[$Hset $Hgood_sl $Hgood_pods $Hgood_frags
       $Hgood_occupied $Hown_pvc_frags $Hoccupied_pvc_frags $Hgood_children
       $Hown_terminating_children_frag $Hreserved_pod_frags $Hreserved_pvc_frags]").
@@ -395,7 +395,7 @@ Proof.
       iAssert (∃ phase, own_terminating_children_frag γ (StatefulSetV.key sts)
           sts.(StatefulSetV.ObjectMeta').(ObjectMetaV.UID') phase)%I
         with "[Hreconcile_Hterminating_children_frag]" as "Hreconcile_Hterminating_children_frag".
-      { iExists (phase_after_deletion Quiescent deletion). iFrame. }
+      { iExists (has_terminating_children_after_deletion terminating_children.No deletion). iFrame. }
       iApply ("HΦ" $! pods' pvcs' interface.nil).
       rewrite /owned_resources /=.
       iFrame "Hown_sts_meta_frag Hown_sts_spec_frag
@@ -420,7 +420,7 @@ Proof.
       iAssert (∃ phase, own_terminating_children_frag γ (StatefulSetV.key sts)
           sts.(StatefulSetV.ObjectMeta').(ObjectMetaV.UID') phase)%I
         with "[Hreconcile_Hterminating_children_frag]" as "Hreconcile_Hterminating_children_frag".
-      { iExists (phase_after_deletion Quiescent deletion). iFrame. }
+      { iExists (has_terminating_children_after_deletion terminating_children.No deletion). iFrame. }
       iApply ("HΦ" $! pods' pvcs' interface.nil).
       rewrite /owned_resources /=.
       iFrame "Hown_sts_meta_frag Hown_sts_spec_frag
@@ -487,7 +487,7 @@ Proof.
     iAssert (∃ phase, own_terminating_children_frag γ (StatefulSetV.key sts)
         sts.(StatefulSetV.ObjectMeta').(ObjectMetaV.UID') phase)%I
       with "[Hreconcile_Hterminating_children_frag]" as "Hreconcile_Hterminating_children_frag".
-    { iExists (phase_after_deletion Quiescent deletion). iFrame. }
+    { iExists (has_terminating_children_after_deletion terminating_children.No deletion). iFrame. }
     iApply ("HΦ" $! pods' pvcs' interface.nil).
     rewrite /owned_resources /=.
     iFrame "Hown_sts_meta_frag Hown_sts_spec_frag
